Start implementing ROBdd API

Bdd.lean
@@ -2,3 +2,138 @@
 -- Import modules here that should be built as part of the library.
 import Bdd.Basic
 import Bdd.Reduce
+import Bdd.Apply
+open List renaming Vector → Vec
+
+-- TODO: this is similar to `OBdd.reachable_or_eq_low_high`
+lemma Pointer.Reachable_iff {heap : Vec (Node n m) m } : Pointer.Reachable heap root p ↔ (p = root ∨ (∃ j, root = .node j ∧ (Pointer.Reachable heap heap[j].low p ∨ Pointer.Reachable heap heap[j].high p))) := by
+  constructor
+  · intro h
+    cases Relation.reflTransGen_swap.mp h with
+    | refl =>
+      left
+      rfl
+    | tail r e =>
+      rename_i q
+      right
+      cases e with
+      | low  hh => rename_i j; exact ⟨j, rfl, .inl (by trans q; rw [hh]; left; exact (Relation.reflTransGen_swap.mpr r))⟩
+      | high hh => rename_i j; exact ⟨j, rfl, .inr (by trans q; rw [hh]; left; exact (Relation.reflTransGen_swap.mpr r))⟩
+  · intro h
+    cases h with
+    | inl h => rw [h]; left
+    | inr h =>
+      rcases h with ⟨j, hj, h⟩
+      rw [hj]
+      cases h with
+      | inl h =>
+        apply Relation.reflTransGen_swap.mp
+        right
+        · apply Relation.reflTransGen_swap.mpr; exact h
+        · left; rfl
+      | inr h =>
+        apply Relation.reflTransGen_swap.mp
+        right
+        · apply Relation.reflTransGen_swap.mpr; exact h
+        · right; rfl
+
+lemma Pointer.eq_terminal_of_reachable : Pointer.Reachable w (.terminal b) p → p = (.terminal b) := by
+  intro h
+  cases Relation.reflTransGen_swap.mp h with
+  | refl => rfl
+  | tail => contradiction
+
+def ROBdd n m := { O : OBdd n m // O.Reduced }
+
+namespace ROBdd
+
+def const : Bool → ROBdd 0 0 := fun b ↦
+  ⟨⟨⟨⟨[], rfl⟩, .terminal b⟩, Bdd.Ordered_of_terminal⟩, OBdd.reduced_of_terminal ⟨b, rfl⟩⟩
+
+def var (n : Nat) : ROBdd n.succ 1 :=
+  ⟨⟨⟨⟨[⟨n, .terminal false, .terminal true⟩], rfl⟩, .node 0⟩,
+  (Ordered_of_Proper (fun N h ↦
+    by
+      simp only [Vec.instMembership, Function.comp_apply, List.Vector.toList_singleton, List.Vector.head, List.mem_cons, List.not_mem_nil, or_false] at h
+      rw [h]
+      intro j hj
+      simp only [reduceCtorEq, or_self] at hj))⟩,
+  ⟨NoRedundancy_of_RProper (fun N h ↦
+    by
+      simp only [Vec.instMembership, Function.comp_apply, List.Vector.toList_singleton, List.Vector.head, List.mem_cons, List.not_mem_nil, or_false] at h
+      rw [h]
+      simp),
+    by
+      rintro ⟨x, hx⟩ ⟨y, hy⟩ h
+      cases Pointer.Reachable_iff.mp hx with
+      | inl hh =>
+        simp only at hh
+        cases Pointer.Reachable_iff.mp hy with
+        | inl hhh =>
+          simp only at hhh
+          simp_rw [hh, hhh]
+          simp [InvImage]
+        | inr hhh =>
+          rcases hhh with ⟨j, hj, hhh⟩
+          simp only at hj
+          injection hj
+          rcases hhh with hhh | hhh <;>
+          simp only [Nat.succ_eq_add_one, Fin.natCast_eq_last, Fin.getElem_fin, Fin.val_eq_zero, Vec.getElem_def, List.Vector.toList_singleton, List.Vector.head, List.getElem_cons_zero] at hhh <;>
+          apply Pointer.eq_terminal_of_reachable at hhh <;>
+          simp_rw [hh, hhh] at h <;>
+          simp only [OBdd.GraphIsomorphic, OBdd.Isomorphic, InvImage] at h <;>
+          unfold OBdd.toTree at h <;>
+          simp at h
+      | inr hh =>
+        simp only at hh
+        rcases hh with ⟨j, hj, hh⟩
+        injection hj
+        simp only [Nat.succ_eq_add_one, Fin.natCast_eq_last, Fin.getElem_fin, Fin.val_eq_zero, Vec.getElem_def, List.Vector.toList_singleton, List.Vector.head, List.getElem_cons_zero] at hh
+        cases Pointer.Reachable_iff.mp hy with
+        | inl hhh =>
+          simp only at hhh
+          rcases hh with hh | hh <;>
+          apply Pointer.eq_terminal_of_reachable at hh <;>
+          simp_rw [hh, hhh] at h <;>
+          simp only [OBdd.GraphIsomorphic, OBdd.Isomorphic, InvImage] at h <;>
+          unfold OBdd.toTree at h <;>
+          simp at h
+        | inr hhh =>
+          simp only at hhh
+          rcases hhh with ⟨i, hi, hhh⟩
+          injection hi
+          simp only [Nat.succ_eq_add_one, Fin.natCast_eq_last, Fin.getElem_fin, Fin.val_eq_zero, Vec.getElem_def, List.Vector.toList_singleton, List.Vector.head, List.getElem_cons_zero] at hhh
+          cases hh with
+          | inl hh =>
+            cases hhh with
+            | inl hhh =>
+              apply Pointer.eq_terminal_of_reachable at hh
+              apply Pointer.eq_terminal_of_reachable at hhh
+              simp [InvImage]
+              rw [hh, hhh]
+            | inr hhh =>
+              apply Pointer.eq_terminal_of_reachable at hh
+              apply Pointer.eq_terminal_of_reachable at hhh
+              simp_rw [hh, hhh] at h
+              simp only [OBdd.GraphIsomorphic, OBdd.Isomorphic, InvImage] at h
+              unfold OBdd.toTree at h
+              simp at h
+          | inr hh =>
+            cases hhh with
+            | inl hhh =>
+              apply Pointer.eq_terminal_of_reachable at hh
+              apply Pointer.eq_terminal_of_reachable at hhh
+              simp_rw [hh, hhh] at h
+              simp only [OBdd.GraphIsomorphic, OBdd.Isomorphic, InvImage] at h
+              unfold OBdd.toTree at h
+              simp at h
+            | inr hhh =>
+              apply Pointer.eq_terminal_of_reachable at hh
+              apply Pointer.eq_terminal_of_reachable at hhh
+              simp [InvImage]
+              rw [hh, hhh]
+          ⟩⟩
+
+-- def not : ROBdd n m → ROBdd n m
+
+end ROBdd
